Checks.lean
@@ -5,6 +5,7 @@ import Checks.Bls12381Conformance
 import Checks.Bls12381Fp
 import Checks.Bls12381Fp2
 import Checks.Bls12381Fp6
+import Checks.Bls12381Fp12
 import Checks.Modexp
 import Checks.Ripemd160
 import Checks.Sha256
